Add mutually recursive types to Lambda (#333)
*Description of changes:*
Adds mutually recursive types to Lambda and its corresponding SMT
generation (`declare-datatypes`). In particular, mutually recursive
types generate multiple eliminators, which still have the expected
computational behavior. This PR includes tests in
`TypeFactoryTests.lean` for eliminators, other derived functions, and
typechecking and in `SMTEncoderDatatypeTest.lean` and
`DatatypeVerificationTest.lean` for SMT output and verification.
Some key changes:
1. Core declarations can now have multiple declarations (and likewise
multiple names)
2. The SMT output becomes simpler. We no longer need dependency analysis
to rule out mutually recursive types, instead checking type references
when a mutual block is created and therefore maintaining a topological
order.
3. Substantial changes to the proofs in `ProgramWF.lean`, which now have
more structure but also more repetition. They can/should be improved in
a future PR.


By submitting this pull request, I confirm that you can use, modify,
copy, and redistribute this contribution, under the terms of your
choice.

---------

Co-authored-by: Josh Cohen <cohenjo@amazon.com>

Strata/DL/Lambda/Identifiers.lean
@@ -70,6 +70,9 @@ def Identifiers.addWithError {IDMeta} (m: Identifiers IDMeta) (x: Identifier IDM
   let (b, m') := m.containsThenInsertIfNew x.name x.metadata
   if b then .error f else .ok m'
 
+def Identifiers.addListWithError {IDMeta} (m: Identifiers IDMeta) (x: List (Identifier IDMeta)) (f: Identifier IDMeta → Format) :=
+  x.foldlM (fun m x => Identifiers.addWithError m x (f x)) m
+
 def Identifiers.add {IDMeta} (m: Identifiers IDMeta) (x: Identifier IDMeta) : Except Format (Identifiers IDMeta) :=
   m.addWithError x f!"Error: duplicate identifier {x.name}"
 
@@ -104,6 +107,48 @@ theorem Identifiers.addWithErrorContains {IDMeta} [DecidableEq IDMeta] {m m': Id
   constructor
   . intros _; apply Or.inl; cases x; cases y; grind
   . rw[meta_eq]; intros _; simp
+
+theorem Identifiers.addListWithErrorNotin {IDMeta} [DecidableEq IDMeta] {m m': Identifiers IDMeta} {l: List (Identifier IDMeta)} {f: Identifier IDMeta → Format}: m.addListWithError l f = .ok m' → forall x, x ∈ l → m.contains x = false := by
+  unfold addListWithError
+  induction l generalizing m m' with
+  | nil => simp
+  | cons h t IH =>
+    simp only[List.foldlM, bind, Except.bind]
+    split <;> intros Hid; try contradiction
+    intros x
+    rw[List.mem_cons]
+    rename_i Heq
+    have Hin := Identifiers.addWithErrorNotin Heq
+    have := addWithErrorContains Heq x; grind
+
+theorem Identifiers.addListWithErrorContains {IDMeta} [DecidableEq IDMeta] {m m': Identifiers IDMeta} {l: List (Identifier IDMeta)} {f: Identifier IDMeta → Format}: m.addListWithError l f = .ok m' → ∀ y, m'.contains y ↔ y ∈ l ∨ m.contains y := by
+  unfold addListWithError
+  induction l generalizing m m' with
+  | nil => simp; intros Heq; cases Heq; grind
+  | cons h t IH =>
+    simp only[List.foldlM, bind, Except.bind]
+    split <;> intros Hid; try contradiction
+    intros x
+    rw[List.mem_cons]
+    rename_i Heq
+    have Hcont := Identifiers.addWithErrorContains Heq x
+    have Hin := Identifiers.addWithErrorNotin Heq
+    grind
+
+theorem Identifiers.addListWithErrorNoDup {IDMeta} [DecidableEq IDMeta] {m m': Identifiers IDMeta} {l: List (Identifier IDMeta)} {f: Identifier IDMeta → Format}: m.addListWithError l f = .ok m' → l.Nodup := by
+  unfold addListWithError
+  induction l generalizing m m' with
+  | nil => simp
+  | cons h t IH =>
+    simp only[List.foldlM, bind, Except.bind]
+    split <;> intros Hid; try contradiction
+    apply List.nodup_cons.mpr
+    constructor <;> try grind
+    intros h_in_t
+    rename_i Hadd
+    have := Identifiers.addWithErrorContains Hadd h
+    have := Identifiers.addListWithErrorNotin Hid h
+    grind
 
 instance [ToFormat IDMeta] : ToFormat (Identifiers IDMeta) where
   format m := format (m.toList)
